Update Stack to the new interface, modulo a problem with the new locks.  Also still need to figure out refinement.

ironfleet/src/Dafny/Distributed/Concur/Stack.i.dfy
@@ -10,8 +10,9 @@ module Stack {
 
     predicate IsValidStack(s:Stack)
     {
-        IsValidLock(s.lock)
-     && IsValidPtr(s.count)
+//        IsValidLock(s.lock)
+//     && 
+        IsValidPtr(s.count)
      && IsValidArray(s.buffers)
      && PtrInvariant(s.count) == iset i | 0 <= i <= s.buffers_len
      && Length(s.buffers) == s.buffers_len
@@ -20,100 +21,86 @@ module Stack {
 
     }
 
-    predicate StackInit(s:Stack, thread_id:int, events:seq<Event>)
+    predicate StackInit(s:Stack, events:seq<Event>)
     {
         s.s == []
-     && events == [ SharedStateEvent(MakeLockEvent(thread_id, s.lock)),
-                    SharedStateEvent(MakePtrEvent(thread_id, ToUPtr(s.count), ToU(0))),
-                    SharedStateEvent(MakeArrayEvent(thread_id, ToUArray(s.buffers), ToU([1,2,3]))) ]
+     && events == [ MakeLockEvent(s.lock),
+                    MakePtrEvent(ToUPtr(s.count), ToU(0)),
+                    MakeArrayEvent(ToUArray(s.buffers), 3, ToU(1)) ]
 
                 
     }
 
-    predicate StackPush(s:Stack, s':Stack, b:Buffer, count:int, thread_id:int, events:seq<Event>)
+    predicate StackPush(s:Stack, s':Stack, b:Buffer, count:int, events:seq<Event>)
     {
         s'.s == s.s + [b]
-     && events == [ SharedStateEvent(LockEvent      (thread_id, s.lock)),
-                    SharedStateEvent(ReadPtrEvent   (thread_id, ToUPtr(s.count), ToU(count))),
-                    SharedStateEvent(WritePtrEvent  (thread_id, ToUPtr(s.count), ToU(count+1))),
-                    SharedStateEvent(WriteArrayEvent(thread_id, ToUArray(s.buffers), count, ToU(b))),
-                    SharedStateEvent(UnlockEvent    (thread_id, s.lock)) ]
+     && events == [ LockEvent      (s.lock),
+                    ReadPtrEvent   (ToUPtr(s.count), ToU(count)),
+                    WritePtrEvent  (ToUPtr(s.count), ToU(count+1)),
+                    WriteArrayEvent(ToUArray(s.buffers), count, ToU(b)),
+                    UnlockEvent    (s.lock) ]
     }
 
-    predicate StackPop(s:Stack, s':Stack, b:Buffer, count:int, thread_id:int, events:seq<Event>)
+    predicate StackPop(s:Stack, s':Stack, b:Buffer, count:int, events:seq<Event>)
     {
         |s.s| > 0
      && s'.s == s.s[..|s.s|-1] 
-     && events == [ SharedStateEvent(LockEvent      (thread_id, s.lock)),
-                    SharedStateEvent(ReadPtrEvent   (thread_id, ToUPtr(s.count), ToU(count))),
-                    SharedStateEvent(WritePtrEvent  (thread_id, ToUPtr(s.count), ToU(count-1))),
-                    SharedStateEvent(ReadArrayEvent (thread_id, ToUArray(s.buffers), count-1, ToU(b))),
-                    SharedStateEvent(UnlockEvent    (thread_id, s.lock)) ]
+     && events == [ LockEvent      (s.lock),
+                    ReadPtrEvent   (ToUPtr(s.count), ToU(count)),
+                    WritePtrEvent  (ToUPtr(s.count), ToU(count-1)),
+                    ReadArrayEvent (ToUArray(s.buffers), count-1, ToU(b)),
+                    UnlockEvent    (s.lock) ]
     }
 
-    predicate StackNoOp(s:Stack, s':Stack, count:int, thread_id:int, events:seq<Event>)
+    predicate StackNoOp(s:Stack, s':Stack, count:int, events:seq<Event>)
     {
         s == s'
-     && events == [ SharedStateEvent(LockEvent   (thread_id, s.lock)),
-                    SharedStateEvent(ReadPtrEvent(thread_id, ToUPtr(s.count), ToU(count))),
-                    SharedStateEvent(UnlockEvent (thread_id, s.lock)) ] 
+     && events == [ LockEvent   (s.lock),
+                    ReadPtrEvent(ToUPtr(s.count), ToU(count)),
+                    UnlockEvent (s.lock) ] 
     }
 
     method MakeStack(ghost env:HostEnvironment, ghost stack_invariant:StackInvariant) returns (s:Stack, ghost events:seq<Event>)
         requires env != null && env.Valid();
-        modifies env.shared;
         modifies env.events;
+        modifies env.locks;
         ensures  IsValidStack(s);
         ensures  s.s == [];
-        ensures  StackInit(s, env.thread.ThreadId(), events);
+        ensures  StackInit(s, events);
         ensures  forall b :: b in s.s ==> b in stack_invariant;
         ensures  env.events.history() == old(env.events.history()) + events;
-//        ensures  var old_heap := old(env.shared.heap());
-//                 var new_heap :=     env.shared.heap() ;
-//                 ToU(s.lock) !in old_heap && ToU(s.count) !in old_heap && ToU(s.buffers) !in old_heap
-//              && ToU(s.lock)  in new_heap && ToU(s.count)  in new_heap && ToU(s.buffers)  in new_heap // All shared objects in s are fresh
-//              && (forall ref :: ref in old_heap ==> ref in new_heap);
     {
-        ghost var thread_id := env.thread.ThreadId();
-
         var lock := SharedStateIfc.MakeLock(env);
 //        ghost var event := env.events.history();
-//        assert event == old(env.events.history()) +  [ SharedStateEvent(MakeLockEvent(thread_id, lock)) ];
+//        assert event == old(env.events.history()) +  [ MakeLockEvent(lock) ];
 
         var count := SharedStateIfc.MakePtr(0, iset i | 0 <= i <= 3, env);
-        assert ToU(count) in env.shared.heap();
 
 //        ghost var event' := env.events.history();
-//        assert event' == event + [SharedStateEvent(MakePtrEvent(thread_id, ToUPtr(count), ToU(0)))];
+//        assert event' == event + [MakePtrEvent(ToUPtr(count), ToU(0))];
 
-        var init := new Buffer[3];
-        init[0] := 1;
-        init[1] := 2;
-        init[2] := 3;
-
-        var buffers := SharedStateIfc.MakeArray(init, iset i | i >= 0, env);
+        var buffers := SharedStateIfc.MakeArray(3, 1, iset i | i >= 0, env);
 //        ghost var event'' := env.events.history();
-//        assert event'' == event' + [SharedStateEvent(MakeArrayEvent(thread_id, ToUArray(buffers), ToU(init[..])))];
-        assert init[..] == [1,2,3];     // OBSERVE: Seq extensionality
-
+//        assert event'' == event' + [MakeArrayEvent(ToUArray(buffers), ToU(init[..]))];
         s := Stack(lock, count, buffers, 3, []);
 
-        events := [ SharedStateEvent(MakeLockEvent(thread_id, s.lock)),
-                    SharedStateEvent(MakePtrEvent(thread_id, ToUPtr(s.count), ToU(0))),
-                    SharedStateEvent(MakeArrayEvent(thread_id, ToUArray(s.buffers), ToU([1,2,3]))) ];
+        events := [ MakeLockEvent(s.lock),
+                    MakePtrEvent(ToUPtr(s.count), ToU(0)),
+                    MakeArrayEvent(ToUArray(s.buffers), 3, ToU(1)) ];
     }
 
     method PushStack(s:Stack, v:Buffer, ghost env:HostEnvironment) returns (s':Stack, ok:bool, ghost count:int, ghost events:seq<Event>)
         requires IsValidStack(s);
         requires v in ArrayInvariant(s.buffers); 
         requires env != null && env.Valid();
-        modifies env.shared;
         modifies env.events;
-        ensures  if ok then StackPush(s, s', v, count, env.thread.ThreadId(), events) 
-                 else StackNoOp(s, s', count, env.thread.ThreadId(), events);
+        modifies env.locks;
+        ensures  if ok then StackPush(s, s', v, count, events) 
+                 else StackNoOp(s, s', count, events);
         ensures  env.events.history() == old(env.events.history()) + events;
     {
-        ghost var thread_id := env.thread.ThreadId();
+        assume s.lock in env.locks.lock_states();     // TODO: Annoying to have to incorporate this into IsValidStack
+        assume !env.locks.lock_states()[s.lock]; 
 
         SharedStateIfc.Lock(s.lock, env);
 
@@ -130,16 +117,16 @@ module Stack {
             ok := true;
             s' := s'.(s := s.s + [v]);
 
-            events := [ SharedStateEvent(LockEvent  (thread_id, s.lock)),
-                        SharedStateEvent(ReadPtrEvent(thread_id, ToUPtr(s.count), ToU(count))),
-                        SharedStateEvent(WritePtrEvent(thread_id, ToUPtr(s.count), ToU(count+1))),
-                        SharedStateEvent(WriteArrayEvent(thread_id, ToUArray(s.buffers), count, ToU(v))),
-                        SharedStateEvent(UnlockEvent(thread_id, s.lock)) ];
+            events := [ LockEvent  (s.lock),
+                        ReadPtrEvent(ToUPtr(s.count), ToU(count)),
+                        WritePtrEvent(ToUPtr(s.count), ToU(count+1)),
+                        WriteArrayEvent(ToUArray(s.buffers), count, ToU(v)),
+                        UnlockEvent(s.lock) ];
         } else {
             ok := false;
-            events := [ SharedStateEvent(LockEvent  (thread_id, s.lock)),
-                        SharedStateEvent(ReadPtrEvent(thread_id, ToUPtr(s.count), ToU(count))),
-                        SharedStateEvent(UnlockEvent(thread_id, s.lock)) ];
+            events := [ LockEvent  (s.lock),
+                        ReadPtrEvent(ToUPtr(s.count), ToU(count)),
+                        UnlockEvent(s.lock) ];
         }
         SharedStateIfc.Unlock(s.lock, env);
     }
@@ -147,14 +134,15 @@ module Stack {
     method PopStack(s:Stack, ghost env:HostEnvironment) returns (s':Stack, v:Buffer, ok:bool, ghost count:int, ghost events:seq<Event>)
         requires IsValidStack(s);
         requires env != null && env.Valid();
-        modifies env.shared;
         modifies env.events;
+        modifies env.locks;
         ensures  ok ==> v in ArrayInvariant(s.buffers); 
-        ensures  if ok then StackPop(s, s', v, count, env.thread.ThreadId(), events) 
-                 else s.s == [] && StackNoOp(s, s', count, env.thread.ThreadId(), events);
+        ensures  if ok then StackPop(s, s', v, count, events) 
+                 else s.s == [] && StackNoOp(s, s', count, events);
         ensures  env.events.history() == old(env.events.history()) + events;
     {
-        ghost var thread_id := env.thread.ThreadId();
+        assume s.lock in env.locks.lock_states();     // TODO: Annoying to have to incorporate this into IsValidStack
+        assume !env.locks.lock_states()[s.lock]; 
 
         SharedStateIfc.Lock(s.lock, env);
 
@@ -168,17 +156,17 @@ module Stack {
             assert Length(s.buffers) == s.buffers_len;  // TODO: Why is this necessary!?
             v := SharedStateIfc.ReadArray(s.buffers, count_impl-1, env);
             ok := true;
-            events := [ SharedStateEvent(LockEvent  (thread_id, s.lock)),
-                        SharedStateEvent(ReadPtrEvent(thread_id, ToUPtr(s.count), ToU(count))),
-                        SharedStateEvent(WritePtrEvent(thread_id, ToUPtr(s.count), ToU(count-1))),
-                        SharedStateEvent(ReadArrayEvent(thread_id, ToUArray(s.buffers), count-1, ToU(v))),
-                        SharedStateEvent(UnlockEvent(thread_id, s.lock)) ];
+            events := [ LockEvent  (s.lock),
+                        ReadPtrEvent(ToUPtr(s.count), ToU(count)),
+                        WritePtrEvent(ToUPtr(s.count), ToU(count-1)),
+                        ReadArrayEvent(ToUArray(s.buffers), count-1, ToU(v)),
+                        UnlockEvent(s.lock) ];
             s' := s'.(s := s.s[..|s.s|-1]); 
         } else {
             ok := false;
-            events := [ SharedStateEvent(LockEvent  (thread_id, s.lock)),
-                        SharedStateEvent(ReadPtrEvent(thread_id, ToUPtr(s.count), ToU(count))),
-                        SharedStateEvent(UnlockEvent(thread_id, s.lock)) ];
+            events := [ LockEvent  (s.lock),
+                        ReadPtrEvent(ToUPtr(s.count), ToU(count)),
+                        UnlockEvent(s.lock) ];
             s' := s;
         }
 
